\documentclass{article}
\usepackage{amsmath,amsfonts,amssymb}
\usepackage{enumitem}
\usepackage[dvipsnames]{xcolor}
\usepackage{multicol}

\setlength{\columnsep}{50pt}

\newlist{multienum}{enumerate}{1}
\setlist[multienum]{
    label=\alph*),
    before=\begin{multicols}{2},
    after=\end{multicols}
}

\newlist{multiitem}{itemize}{1}
\setlist[multiitem]{
    label=\textbullet,
    before=\begin{multicols}{4},
    after=\end{multicols}
}

\title{Trigonometric Identity Proof}
\author{Kensukeken}
\date{January 12, 2024}

\begin{document}
\maketitle

\section{Prove each identity:}
\begin{multicols}{2}
    \begin{enumerate}[label=\alph*.]
        \item $\sin\theta = \tan \theta \cos \theta$
        \begin{align*}
          \text{\textcolor{blue}{LHS}} &= \text{\textcolor{blue}{$\sin\theta$}} \\
          &= \text{\textcolor{blue}{$\frac{\sin\theta}{\cos\theta} \cdot \cos\theta$}} \quad \text{\textcolor{blue}{(Multiplying by $\frac{\cos\theta}{\cos\theta}$)}} \\
          &= \text{\textcolor{blue}{$\tan\theta \cos\theta$}} \quad \text{\textcolor{blue}{(Definition of $\tan\theta$)}}
        \end{align*}
       

        \item $\cos \theta = \frac{\sin\theta}{\tan \theta}$
        \begin{align*}
          \text{\textcolor{blue}{LHS}} &= \text{\textcolor{blue}{$\cos\theta$}} \\
          &= \text{\textcolor{blue}{$\frac{\cos\theta}{\sin\theta} \cdot \sin\theta$}} \quad \text{\textcolor{blue}{(Multiplying by $\frac{\sin\theta}{\sin\theta}$)}} \\
          &= \text{\textcolor{blue}{$\frac{\sin\theta}{\tan\theta}$}} \quad \text{\textcolor{blue}{(Definition of $\tan\theta$)}}
        \end{align*}
    \end{enumerate}
\end{multicols}

\section{Prove each identity:}
\begin{multienum}
    \item $\frac{1}{\sin \theta}(1+ \sin \theta)=1+\frac{1}{\sin \theta}$
    \begin{align*}
        \text{\textcolor{blue}{LHS}} &= \frac{1}{\sin \theta}(1+ \sin \theta) \\
        &= \frac{1}{\sin \theta} + 1 \\
        &= 1 + \frac{1}{\sin \theta} \quad (\text{\textcolor{blue}{RHS}})
    \end{align*}

    \item $\sin \theta \left( 1+ \frac{1}{\sin \theta }\right)=1+ \sin \theta$
    \begin{align*}
        \text{\textcolor{blue}{LHS}} &= \sin \theta \left( 1+ \frac{1}{\sin \theta }\right) \\
        &= \sin \theta + 1 \\
        &= 1 + \sin \theta \quad (\text{\textcolor{blue}{RHS}})
    \end{align*}

    \item $\cos \left( \frac{1}{\cos \theta -1}\right)=1- \cos \theta$
    \begin{align*}
        \text{\textcolor{blue}{LHS}} &= \cos \left( \frac{1}{\cos \theta -1}\right) \\
        &= 1 - \cos \theta \quad (\text{\textcolor{blue}{RHS}})
    \end{align*}

    \item $\frac{\sin \theta }{\cos \theta \tan \theta} = 1$
    \begin{align*}
        \text{\textcolor{blue}{LHS}} &= \frac{\sin \theta }{\cos \theta \tan \theta} \\
        &= \frac{\sin \theta }{\frac{\sin \theta }{\cos \theta}} \\
        &= \cos \theta \quad (\text{\textcolor{blue}{RHS}})
    \end{align*}
\end{multienum}
\newpage 
\section{Knowledge/Understadning }
\begin{multienum}
    \item $\tan^2 \theta = \frac{1 - \cos^2 \theta}{\cos^2 \theta}$
    \begin{align*}
        \text{\textcolor{blue}{LHS}} &= \tan^2 \theta \\
        &= \frac{\sin^2 \theta}{\cos^2 \theta} \\
        &= \frac{1 - \cos^2 \theta}{\cos^2 \theta} \quad (\text{\textcolor{blue}{RHS}})
    \end{align*}

    \item $\sin \theta \tan \theta = \frac{1 - \cos^2 \theta}{\cos \theta}$
    \begin{align*}
        \text{\textcolor{blue}{LHS}} &= \sin \theta \tan \theta \\
        &= \frac{\sin^2 \theta}{\cos \theta} \\
        &= \frac{1 - \cos^2 \theta}{\cos \theta} \quad (\text{\textcolor{blue}{RHS}})
    \end{align*}

    \item $\frac{\sin \theta}{1 + \cos \theta} = \frac{1 - \cos \theta}{\sin \theta}$
    \begin{align*}
        \text{\textcolor{blue}{LHS}} &= \frac{\sin \theta}{1 + \cos \theta} \\
        &= \frac{1 - \cos \theta}{\sin \theta} \quad (\text{\textcolor{blue}{RHS}})
    \end{align*}

    \item $1 - \tan \theta = -\tan \theta \left(1 - \frac{1}{\tan \theta} \right)$
    \begin{align*}
        \text{\textcolor{blue}{LHS}} &= 1 - \tan \theta \\
        &= -\tan \theta \left(1 - \frac{1}{\tan \theta} \right) \quad (\text{\textcolor{blue}{RHS}})
    \end{align*}
\end{multienum}

\section{Prove each identity:}
\begin{multienum}
    \item $\sin \theta \tan \theta+\frac{1}{\cos \theta}=\frac{\sin ^2 \theta+1}{\cos \theta}$
    \begin{align*}
        \text{\textcolor{blue}{LHS}} &= \sin \theta \tan \theta+\frac{1}{\cos \theta} \\
        &= \frac{\sin^2 \theta}{\cos \theta}+\frac{1}{\cos \theta} \\
        &= \frac{\sin ^2 \theta+1}{\cos \theta} \quad (\text{\textcolor{blue}{RHS}})
    \end{align*}

    \item $\frac{1+\cos \theta}{1-\cos \theta}=\frac{1+\frac{1}{\cos \theta}}{\frac{1}{\cos \theta}-1}$
    \begin{align*}
        \text{\textcolor{blue}{LHS}} &= \frac{1+\cos \theta}{1-\cos \theta} \\
        &= \frac{\frac{1}{\cos \theta}(\cos \theta+1)}{\frac{1}{\cos \theta}(\cos \theta-1)} \\
        &= \frac{1+\frac{1}{\cos \theta}}{\frac{1}{\cos \theta}-1} \quad (\text{\textcolor{blue}{RHS}})
    \end{align*}

    \item $\frac{1+\sin \theta}{1-\sin \theta}=\frac{\frac{1}{\sin \theta}+1}{\frac{1}{\sin \theta}-1}$
    \begin{align*}
        \text{\textcolor{blue}{LHS}} &= \frac{1+\sin \theta}{1-\sin \theta} \\
        &= \frac{\frac{1}{\sin \theta}(\sin \theta+1)}{\frac{1}{\sin \theta}(\sin \theta-1)} \\
        &= \frac{\frac{1}{\sin \theta}+1}{\frac{1}{\sin \theta}-1} \quad (\text{\textcolor{blue}{RHS}})
    \end{align*}

    \item $\left(\frac{1}{\cos \theta}+\tan \theta\right)(1-\sin \theta)=\cos \theta$
    \begin{align*}
        \text{\textcolor{blue}{LHS}} &= \left(\frac{1}{\cos \theta}+\tan \theta\right)(1-\sin \theta) \\
        &= \frac{1-\sin \theta}{\cos \theta}(\cos \theta) \\
        &= \cos \theta \quad (\text{\textcolor{blue}{RHS}})
    \end{align*}
\end{multienum}

\section{Prove each identity:}
\begin{multienum}
    \item $\frac{\sin ^2 \theta}{\tan ^2 \theta}=1-\sin ^2 \theta$
    \begin{align*}
        \text{\textcolor{blue}{LHS}} &= \frac{\sin ^2 \theta}{\tan ^2 \theta} \\
        &= \frac{\sin ^2 \theta}{\frac{\sin ^2 \theta}{\cos ^2 \theta}} \\
        &= 1-\sin ^2 \theta \quad (\text{\textcolor{blue}{RHS}})
    \end{align*}

    \item $\frac{1}{\sin ^2 \theta}-1=\frac{\cos ^2 \theta}{\sin ^2 \theta}$
    \begin{align*}
        \text{\textcolor{blue}{LHS}} &= \frac{1}{\sin ^2 \theta}-1 \\
        &= \frac{\cos ^2 \theta}{\sin ^2 \theta} \quad (\text{\textcolor{blue}{RHS}})
    \end{align*}

    \item $\sin ^2 \theta=\frac{\tan ^2 \theta}{1+\tan ^2 \theta}$
    \begin{align*}
        \text{\textcolor{blue}{LHS}} &= \sin ^2 \theta \\
        &= \frac{\tan ^2 \theta}{1+\tan ^2 \theta} \quad (\text{\textcolor{blue}{RHS}})
    \end{align*}

    \item $\sin \theta+\frac{\cos \theta}{\tan \theta}=\frac{1}{\cos \theta \tan \theta}$
    \begin{align*}
        \text{\textcolor{blue}{LHS}} &= \sin \theta+\frac{\cos \theta}{\tan \theta} \\
        &= \frac{\sin \theta \cos \theta}{\sin \theta} \\
        &= \frac{1}{\cos \theta \tan \theta} \quad (\text{\textcolor{blue}{RHS}})
    \end{align*}
\end{multienum}

\section{Application}
\begin{multienum}
    \item Prove this identity.
    $$
    \sin \theta+\cos \theta=\sin \theta \cos \theta\left(\frac{1}{\sin \theta}+\frac{1}{\cos \theta}\right)
    $$
    \begin{align*}
        \text{\textcolor{blue}{LHS}} &= \sin \theta+\cos \theta \\
        &= \sin \theta \cos \theta\left(\frac{1}{\sin \theta}+\frac{1}{\cos \theta}\right) \quad (\text{\textcolor{blue}{RHS}})
    \end{align*}

    \item Prove this identity.
    $$
    \tan ^2 \theta=\left(\frac{1}{\cos \theta}-1\right)\left(\frac{1}{\cos \theta}+1\right)
    $$
    \begin{align*}
        \text{\textcolor{blue}{LHS}} &= \tan ^2 \theta \\
        &= \left(\frac{1}{\cos \theta}-1\right)\left(\frac{1}{\cos \theta}+1\right) \quad (\text{\textcolor{blue}{RHS}})
    \end{align*}
\end{multienum}

\section{Prove each identity:}
\begin{multienum}
    \item $\tan \theta+\frac{1}{\tan \theta}=\frac{1}{\sin \theta \cos \theta}$
    \begin{align*}
        \text{\textcolor{blue}{LHS}} &= \tan \theta+\frac{1}{\tan \theta} \\
        &= \frac{1}{\sin \theta \cos \theta} \quad (\text{\textcolor{blue}{RHS}})
    \end{align*}

    \item $\frac{\sin \theta}{1+\cos \theta}+\frac{1+\cos \theta}{\sin \theta}=\frac{2}{\sin \theta}$
    \begin{align*}
        \text{\textcolor{blue}{LHS}} &= \frac{\sin \theta}{1+\cos \theta}+\frac{1+\cos \theta}{\sin \theta} \\
        &= \frac{2}{\sin \theta} \quad (\text{\textcolor{blue}{RHS}})
    \end{align*}

    \item $\tan \theta+\frac{\cos \theta}{1+\sin \theta}=\frac{1}{\cos \theta}$
    \begin{align*}
        \text{\textcolor{blue}{LHS}} &= \tan \theta+\frac{\cos \theta}{1+\sin \theta} \\
        &= \frac{1}{\cos \theta} \quad (\text{\textcolor{blue}{RHS}})
    \end{align*}

    \item $\frac{\tan \theta-\sin \theta}{\sin ^3 \theta}=\frac{1}{\cos \theta(1+\cos \theta)}$
    \begin{align*}
        \text{\textcolor{blue}{LHS}} &= \frac{\tan \theta-\sin \theta}{\sin ^3 \theta} \\
        &= \frac{1}{\cos \theta(1+\cos \theta)} \quad (\text{\textcolor{blue}{RHS}})
    \end{align*}
\end{multienum}

\end{document}
