\documentclass{article}
\usepackage{amsmath}
\usepackage{amsmath}

\begin{document}
\title{Harcourt Homework}
\maketitle
\section*{Mon - Nov 13 Pg \# 44 1-6}
\section*{PART A}

\subsection*{1. Evaluate the following:}

a. $\sqrt{121}$
\begin{align*}
    \sqrt{121} 
    &= 11
\end{align*}

b. $\sqrt{625}$
\begin{align*}
    \sqrt{625} &= 25
\end{align*}

c. $\sqrt{\frac{4}{9}}$
\begin{align*}
    \sqrt{\frac{4}{9}} &= \frac{2}{3}
\end{align*}

d. $\sqrt{0.01}$
\begin{align*}
    \sqrt{0.01} &= 0.1
\end{align*}

e. $\sqrt{2 \frac{1}{4}}$
\begin{align*}
    \sqrt{2 \frac{1}{4}} &= \sqrt{\frac{9}{4}} \\
    &= \frac{3}{2}
\end{align*}

f. $\sqrt{25-16}$
\begin{align*}
    \sqrt{25-16} &= \sqrt{9} \\
    &= 3
\end{align*}

g. $\sqrt{100}-\sqrt{36}$
\begin{align*}
    \sqrt{100}-\sqrt{36} &= 10 - 6 \\
    &= 4
\end{align*}

h. $(\frac{V}{7})^2$
\begin{align*}
    \left(\frac{V}{7}\right)^2 &= \frac{V^2}{49}
\end{align*}

\subsection*{2. Simplify the following:}

a. $\sqrt{5} \times \sqrt{7}$
\begin{align*}
    \sqrt{5} \times \sqrt{7} &= \sqrt{35}
\end{align*}

b. $2 \sqrt{3} \times 3 \sqrt{5}$
\begin{align*}
    2 \sqrt{3} \times 3 \sqrt{5} &= 6 \sqrt{15}
\end{align*}

c. $3 \sqrt{5}+\sqrt{5}$
\begin{align*}
    3 \sqrt{5}+\sqrt{5} &= 4 \sqrt{5}
\end{align*}

d. $2 \sqrt{7}-5 \sqrt{7}$
\begin{align*}
    2 \sqrt{7}-5 \sqrt{7} &= -3 \sqrt{7}
\end{align*}

e. $2(\sqrt{3}+3)$
\begin{align*}
    2(\sqrt{3}+3) &= 2\sqrt{3}+6
\end{align*}

f. $\sqrt{2}(1 + \sqrt{2})$
\begin{align*}
    \sqrt{2}(1 + \sqrt{2}) &= \sqrt{2} + 2
\end{align*}

g. $3 \sqrt{2}(\sqrt{3}-\sqrt{3})$
\begin{align*}
    3 \sqrt{2}(\sqrt{3}-\sqrt{3}) &= 0
\end{align*}

h. $\sqrt{\frac{\pi}{2}} \times 2 \sqrt{6}$
\begin{align*}
    \sqrt{\frac{\pi}{2}} \times 2 \sqrt{6} &= \sqrt{3\pi}
\end{align*}

\section*{PART B}

\subsection*{3. Change the following to mixed radicals in simplest form:}

a. $\sqrt{12}$
\begin{align*}
    \sqrt{12} &= 2\sqrt{3}
\end{align*}

b. $\sqrt{18}$
\begin{align*}
    \sqrt{18} &= 3\sqrt{2}
\end{align*}

c. $\sqrt{45}$
\begin{align*}
    \sqrt{45} &= 3\sqrt{5}
\end{align*}

d. $\sqrt{75}$
\begin{align*}
    \sqrt{75} &= 5\sqrt{3}
\end{align*}

e. $\sqrt{200}$
\begin{align*}
    \sqrt{200} &= 10\sqrt{2}
\end{align*}

f. $\sqrt{512}$
\begin{align*}
    \sqrt{512} &= 16\sqrt{2}
\end{align*}

g. $3 \sqrt{24}$
\begin{align*}
    3 \sqrt{24} &= 12\sqrt{6}
\end{align*}

h. $5 \sqrt{63}$
\begin{align*}
    5 \sqrt{63} &= 15\sqrt{7}
\end{align*}

i. $9 \sqrt{72}$
\begin{align*}
    9 \sqrt{72} &= 18\sqrt{2}
\end{align*}

j. $3 \sqrt{123}$
\begin{align*}
    3 \sqrt{123} &= 3\sqrt{3}\sqrt{41}
\end{align*}

\subsection*{4. Simplify the following:}

a. $\sqrt{2} \times \sqrt{10}$
\begin{align*}
    \sqrt{2} \times \sqrt{10} &= 2\sqrt{5}
\end{align*}

b. $\sqrt{6} \times \sqrt{8}$
\begin{align*}
    \sqrt{6} \times \sqrt{8} &= 4\sqrt{3}
\end{align*}

c. $\sqrt{5} \times 2 \sqrt{15}$
\begin{align*}
    \sqrt{5} \times 2 \sqrt{15} &= 10\sqrt{3}
\end{align*}

d. $2 \sqrt{3} \times 3 \sqrt{6}$
\begin{align*}
    2 \sqrt{3} \times 3 \sqrt{6} &= 18\sqrt{2}
\end{align*}

e. $\sqrt{6} \times \sqrt{10} \times \sqrt{15}$
\begin{align*}
    \sqrt{6} \times \sqrt{10} \times \sqrt{15} &= 30
\end{align*}

f. $2 \sqrt{5} \times \sqrt{10} \times 3 \sqrt{5}$
\begin{align*}
    2 \sqrt{5} \times \sqrt{10} \times 3 \sqrt{5} &= 20\sqrt{5}
\end{align*}

g. $3 \sqrt{6} \times 6 \sqrt{3} \times \sqrt{2}$
\begin{align*}
    3 \sqrt{6} \times 6 \sqrt{3} \times \sqrt{2} &= 108
\end{align*}

h. $3 \sqrt{7} \times 2 \sqrt{3} \times 2 \sqrt{7}$
\begin{align*}
    3 \sqrt{7} \times 2 \sqrt{3} \times 2 \sqrt{7} &= 12\sqrt{21}
\end{align*}

i. $4 \sqrt{5} \times 3 \sqrt{6} \times 7 \sqrt{5}$
\begin{align*}
    4 \sqrt{5} \times 3 \sqrt{6} \times 7 \sqrt{5} &= 84\sqrt{30}
\end{align*}

\subsection*{5. Simplify the following:}

a. $2 \sqrt{3}-\sqrt{5}-\sqrt{3}+4 \sqrt{5}$
\begin{align*}
    2 \sqrt{3}-\sqrt{5}-\sqrt{3}+4 \sqrt{5} &= 6\sqrt{3}+3\sqrt{5}
\end{align*}

b. $4 \sqrt{7}-7-2 \sqrt{7}-7$
\begin{align*}
    4 \sqrt{7}-7-2 \sqrt{7}-7 &= 2\sqrt{7}-14
\end{align*}

c. $\sqrt{3}+\sqrt{12}$
\begin{align*}
    \sqrt{3}+\sqrt{12} &= 3\sqrt{3}
\end{align*}

d. $4 \sqrt{2}-\sqrt{32}$
\begin{align*}
    4 \sqrt{2}-\sqrt{32} &= 0
\end{align*}

e. $\sqrt{75}-\sqrt{48}$
\begin{align*}
    \sqrt{75}-\sqrt{48} &= \sqrt{3}
\end{align*}

f. $\sqrt{2}+\sqrt{8}+\sqrt{18}$
\begin{align*}
    \sqrt{2}+\sqrt{8}+\sqrt{18} &= 6\sqrt{2}
\end{align*}

g. $3 \sqrt{12}-2 \sqrt{27}$
\begin{align*}
    3 \sqrt{12}-2 \sqrt{27} &= 0
\end{align*}

h. $\sqrt{2}+\sqrt{4}+\sqrt{8}+\sqrt{16}$
\begin{align*}
    \sqrt{2}+\sqrt{4}+\sqrt{8}+\sqrt{16} &= 6+3\sqrt{2}
\end{align*}

i. $2 \sqrt{18}-\sqrt{24}-3 \sqrt{8}$
\begin{align*}
    2 \sqrt{18}-\sqrt{24}-3 \sqrt{8} &= -2\sqrt{6}
\end{align*}

\subsection*{6. Simplify the following:}

a. $\sqrt{5}(\sqrt{5}-\sqrt{10})$
\begin{align*}
    \sqrt{5}(\sqrt{5}-\sqrt{10}) &= 5-5\sqrt{2}
\end{align*}

b. $2 \sqrt{3}(3 \sqrt{2}+\sqrt{3})$
\begin{align*}
    2 \sqrt{3}(3 \sqrt{2}+\sqrt{3}) &= 6\sqrt{6}+6
\end{align*}

c. $3 \sqrt{2}(\sqrt{6}+\sqrt{18})$
\begin{align*}
    3 \sqrt{2}(\sqrt{6}+\sqrt{18}) &= 3\sqrt{12}+18\sqrt{2}
\end{align*}

d. $(2+\sqrt{3})(3+\sqrt{3})$
\begin{align*}
    (2+\sqrt{3})(3+\sqrt{3}) &= 9+5\sqrt{3}
\end{align*}

e. $(3-2 \sqrt{6})(4+\sqrt{6})$
\begin{align*}
    (3-2 \sqrt{6})(4+\sqrt{6}) &= -6-2\sqrt{6}
\end{align*}

f. $(2 \sqrt{5}+3 \sqrt{2})(2 \sqrt{5}-3 \sqrt{2})$
\begin{align*}
    (2 \sqrt{5}+3 \sqrt{2})(2 \sqrt{5}-3 \sqrt{2}) &= 20-12
\end{align*}
\newpage
\section*{Wed - Nov 22, Pg \# 127 1-4, 6}
\section*{PART 1}

\subsection*{1. Change to logarithmic notation, $y=\log _d x$.}

\begin{enumerate}
    \item $3^5=243$
    \[y = \log_3 243\]

    \item $2^7=128$
    \[y = \log_2 128\]

    \item $7^3=343$
    \[y = \log_7 343\]

    \item $11^4=14641$
    \[y = \log_{11} 14641\]
\end{enumerate}

\subsection*{2. Change to exponential notation, $x=a^y$.}

\begin{enumerate}
    \item $\log_4 1024=5$
    \[x = 4^5\]

    \item $\log_7 7=1$
    \[x = 7^1\]

    \item $\log_6 7776=5$
    \[x = 6^5\]

    \item $\log_a p=r$
    \[x = a^r\]
\end{enumerate}

\subsection*{3. Evaluate each of the following.}

\begin{enumerate}
    \item $\log_{10} 100$
    \[\log_{10} 100 = 2\]

    \item $\log_6 216$
    \[\log_6 216 = 3\]

    \item $\log_7 1$
    \[\log_7 1 = 0\]

    \item $\log_4 1024$
    \[\log_4 1024 = 5\]
\end{enumerate}

\subsection*{4. Use calculator to determine each of the following.}

\begin{enumerate}
    \item $\log 327$
    \[\log 327 \approx 2.5132\]

    \item $\log (6^3)$
    \[\log (216) = 2.3345\]

    \item $\log (0.001)$
    \[\log (0.001) = -3\]

    \item $\log (0.039)$
    \[\log (0.039) \approx -1.4082\]
\end{enumerate}

\section*{PART B}

\subsection*{5. Evaluate each of the following.}

\begin{enumerate}
    \item $1.03^{15}$
    \[1.03^{15} \approx 1.495\]

    \item $1.02^{20}$
    \[1.02^{20} \approx 1.485\]

    \item $1.06^{12}$
    \[1.06^{12} \approx 1.923\]

    \item $1.03^{24}$
    \[1.03^{24} \approx 2.036\]
\end{enumerate}

\subsection*{6. Solve for $x$ in each of the following.}

\begin{enumerate}
    \item $3^x=32$
    \[x = \log_3 32 = 5\]

    \item $5^x=66$
    \[x = \frac{\log 66}{\log 5} \approx 3.46\]

    \item $10^x=157$
    \[x = \log 157 \approx 2.20\]

    \item $1.03^x=1.69$
    \[x = \frac{\log 1.69}{\log 1.03} \approx 22.34\]

    \item $4 \cdot 5^x=600$
    \[x = \frac{\log (600/4)}{\log 5} \approx 4.80\]

    \item $1.02^x=3.65$
    \[x = \frac{\log 3.65}{\log 1.02} \approx 216.74\]

    \item $1.05^x=2.60$
    \[x = \frac{\log 2.60}{\log 1.05} \approx 14.65\]

    \item $1.045^x=2.87$
    \[x = \frac{\log 2.87}{\log 1.045} \approx 31.52\]

    \item $\log 1.07^x=2$
    \[x = \frac{2}{\log 1.07} \approx 20.74\]
\end{enumerate}
\end{document}
