\documentclass{article}
\usepackage{amsmath}
\usepackage{amsfonts}
\usepackage{amssymb}
\usepackage{geometry}
\usepackage{enumitem}
\usepackage{cancel}
\geometry{a4paper, margin=1in}

\title{Unit 2 Test - Functions}
\date{}
\begin{document}
\maketitle

\section*{Instructions}
Answer all questions. Show all work. Be sure to simplify your answers when necessary.

\section*{Simplifying Rational Expressions}
\begin{enumerate}
    \item Simplify the following rational expression:
    \begin{equation*}
        \frac{2x^2 - 8x}{4x^3 - 12x^2}
    \end{equation*}
    \begin{align*}
\frac{2x^2 - 8x}{4x^3 - 12x^2} &= \frac{2x(x - 4)}{4x^2(x - 3)} \\
&= \frac{2x(x - 4)}{4x^2(x - 3)} \cdot \frac{1}{2} \quad \text{Divide by 2} \\
&= \frac{x(x - 4)}{2x(x - 3)} \\
\end{align*}

    \item Simplify the following rational expression:
    \begin{equation*}
        \frac{3a^3b^2 - 6a^2b^3}{9a^2b^2 - 12ab^3}
    \end{equation*}
    \begin{align*}
\frac{3a^3b^2 - 6a^2b^3}{9a^2b^2 - 12ab^3} &= \frac{3a^2b^2(a - 2b)}{3ab^2(3a - 4b)} \\
&= \frac{a^2b^2(a - 2b)}{ab^2(3a - 4b)} \\
&= \frac{a(a - 2b)}{3a - 4b} \\
\end{align*}

\end{enumerate}

\section*{Multiplying / Dividing Rational Expressions}
\begin{enumerate}[resume]
    \item Multiply the following rational expressions:
    \begin{equation*}
        \frac{x^2}{3y} \cdot \frac{3y^2}{x}
    \end{equation*}
    \begin{align*}
\frac{x^2}{3y} \cdot \frac{3y^2}{x} &= \frac{x^2 \cdot 3y^2}{3y \cdot x} \\
&= \frac{3x^2y^2}{3xy} \\
&= xy
\end{align*}

    \item Divide the following rational expressions:
    \begin{equation*}
        \frac{4a^3b^2}{12a^2b^4} \div \frac{2a^2b}{6ab^3}
    \end{equation*}

\begin{align*}
\frac{4a^3b^2}{12a^2b^4} \div \frac{2a^2b}{6ab^3} &= \frac{4a^3b^2}{12a^2b^4} \cdot \frac{6ab^3}{2a^2b} \\
&= \frac{4 \cdot 6 \cdot a^3 \cdot b^2 \cdot ab^3}{12 \cdot 2 \cdot a^2 \cdot b^4 \cdot a^2 \cdot b} \\
&= \frac{\cancel{24a^4b^5}}{\cancel{24a^4b^5}} \\
&= 1
\end{align*}

\end{enumerate}

\section*{Adding / Subtracting Rational Expressions}
\begin{enumerate}[resume]
    \item Add or subtract the following rational expressions (as applicable):
    \begin{equation*}
        \frac{2}{x} + \frac{1}{x^2}
    \end{equation*}
    \begin{align*}
\frac{2}{x} + \frac{1}{x^2} &= \frac{2x}{x^2} + \frac{1}{x^2} \\
&= \frac{2x + 1}{x^2}
\end{align*}

    \item Add or subtract the following rational expressions (as applicable):
    \begin{equation*}
        \frac{3}{a^2 - 9} - \frac{2}{a + 3}
    \end{equation*}
    \begin{align*}
\frac{3}{a^2 - 9} - \frac{2}{a + 3} &= \frac{3}{(a + 3)(a - 3)} - \frac{2}{a + 3} \\
&= \frac{3}{(a + 3)(a - 3)} - \frac{2(a - 3)}{(a + 3)(a - 3)} \\
&= \frac{3 - 2a + 6}{(a + 3)(a - 3)} \\
&= \frac{-2a + 9}{(a + 3)(a - 3)}
\end{align*}

\end{enumerate}
\newpage 
\section*{Solving Rational Equations}
\begin{enumerate}[resume]
    \item Solve the following rational equation for $x$:
    \begin{equation*}
        \frac{1}{x} + \frac{2}{x + 3} = \frac{3}{x + 6}
    \end{equation*}
\begin{align*}
\frac{1}{x} + \frac{2}{x + 3} &= \frac{3}{x + 6} \\
\text{To eliminate fractions, we can find a common denominator, which is } x(x + 3)(x + 6): \\
x(x + 6) + 2x(x + 6) &= 3x(x + 3) \\
x(x + 6 + 2x) &= 3x(x + 3) \\
x(x^2 + 6x + 2x) &= 3x(x^2 + 3x) \\
x^3 + 8x^2 &= 3x^3 + 9x^2 \\
x^3 - 3x^3 + 8x^2 - 9x^2 &= 0 \\
-2x^3 - x^2 &= 0 \\
x^2(2x + 1) &= 0 \\
\end{align*}

    
    \item Solve the following rational equation for $a$:
    \begin{equation*}
        \frac{4}{a} = \frac{3}{a - 2}
    \end{equation*}
    \begin{align*}
\frac{4}{a} &= \frac{3}{a - 2} \\
\text{To eliminate fractions, we can cross-multiply:} \\
4(a - 2) &= 3a \\
4a - 8 &= 3a \\
4a - 3a &= 8 \\
a &= 8
\end{align*}

\end{enumerate}
\newpage 
\section*{Word Problems}
\begin{enumerate}[resume]
    \item A group of friends decides to share a cake. If it takes Alice 2 hours to eat the entire cake, Bob 3 hours, and Carol 4 hours, how long will it take them to eat the cake together?
\begin{align*}
\text{Let } t \text{ be the time it takes for all of them to eat the cake together.} \\
\frac{1}{2} + \frac{1}{3} + \frac{1}{4} &= \frac{1}{t} \\
\text{To solve for } t, \text{ find the common denominator:} \\
\frac{6}{12} + \frac{4}{12} + \frac{3}{12} &= \frac{1}{t} \\
\frac{13}{12} &= \frac{1}{t} \\
\text{Take the reciprocal:} \\
t &= \frac{12}{13} \text{ hours}
\end{align*}

    
    \item A car travels at an average speed of 60 mph from city A to city B. On the return trip, the car travels at an average speed of 40 mph. If the total round trip distance is 240 miles, how far is it from city A to city B?
    \begin{align*}
\text{Let } d \text{ be the one-way distance from city A to city B.} \\
\text{Time for the first trip:} \quad \frac{d}{60} \text{ hours} \\
\text{Time for the return trip:} \quad \frac{d}{40} \text{ hours} \\
\text{Total time for the round trip:} \quad \frac{d}{60} + \frac{d}{40} \text{ hours} \\
\text{The total round trip distance is 240 miles, so:} \\
\frac{d}{60} + \frac{d}{40} &= \frac{240}{1} \\
\text{To solve for } d, \text{ find the common denominator:} \\
\frac{4d}{240} + \frac{6d}{240} &= \frac{240}{1} \\
\frac{10d}{240} &= \frac{240}{1} \\
\text{Simplify:} \\
\frac{d}{24} &= \frac{240}{1} \\
\text{Take the reciprocal:} \\
d &= 24 \cdot \frac{1}{240} \\
d &= 0.1 \text{ miles} \text{ (or } 1/10 \text{ mile)}
\end{align*}

\end{enumerate}
\end{document}
